Switch OQL compilation to extended NRA

coq/Frontend/ODMG/OQLtoNRAEnv.v
@@ -24,63 +24,62 @@ Section OQLtoNRAEnv.
   Require Import Utils BasicSystem.
 
   Require Import OQL.
-  Require Import RAlgEnv.
+  Require Import NRAEnv.
 
   Context {fruntime:foreign_runtime}.
 
   Context (h:list(string*string)).
   Context (constant_env:list (string*data)).
 
-
   (*****************************
    * OQL to NRAEnv translation *
    *****************************)
   
-  Fixpoint algenv_of_oql (e:oql_expr) : algenv :=
+  Fixpoint nraenv_of_oql (e:oql_expr) : nraenv :=
     match e with
-    | OConst d => ANConst d
-    | OVar v => ANUnop (ADot v) ANID
-    | OTable t => ANGetConstant t
-    | OBinop b e1 e2 => ANBinop b (algenv_of_oql e1) (algenv_of_oql e2)
-    | OUnop u e1 => ANUnop u (algenv_of_oql e1)
+    | OConst d => NRAEnvConst d
+    | OVar v => NRAEnvUnop (ADot v) NRAEnvID
+    | OTable t => NRAEnvGetConstant t
+    | OBinop b e1 e2 => NRAEnvBinop b (nraenv_of_oql e1) (nraenv_of_oql e2)
+    | OUnop u e1 => NRAEnvUnop u (nraenv_of_oql e1)
     | OSFW select_clause from_clause where_clause order_clause =>
-      let algenv_of_from (opacc:algenv) (from_in_expr : oql_in_expr) :=
+      let nraenv_of_from (opacc:nraenv) (from_in_expr : oql_in_expr) :=
           match from_in_expr with
             | OIn in_v from_expr =>
-              ANMapConcat (ANMap (ANUnop (ARec in_v) ANID) (algenv_of_oql from_expr)) opacc
+              NRAEnvMapConcat (NRAEnvMap (NRAEnvUnop (ARec in_v) NRAEnvID) (nraenv_of_oql from_expr)) opacc
             | OInCast in_v brand_name from_expr =>
-              ANMapConcat (ANMap (ANUnop (ARec in_v) ANID)
-                                 (ANUnop AFlatten
-                                         (ANMap
-                                            (ANEither (ANUnop AColl ANID)
-                                                      (ANConst (dcoll nil)))
-                                            (ANMap (ANUnop (ACast (brand_name::nil)) ANID)
-                                                   (algenv_of_oql from_expr))
+              NRAEnvMapConcat (NRAEnvMap (NRAEnvUnop (ARec in_v) NRAEnvID)
+                                 (NRAEnvUnop AFlatten
+                                         (NRAEnvMap
+                                            (NRAEnvEither (NRAEnvUnop AColl NRAEnvID)
+                                                      (NRAEnvConst (dcoll nil)))
+                                            (NRAEnvMap (NRAEnvUnop (ACast (brand_name::nil)) NRAEnvID)
+                                                   (nraenv_of_oql from_expr))
                                          )))
                           opacc
           end
       in
-      let algenv_of_from_clause :=
-          fold_left algenv_of_from from_clause (ANUnop AColl ANID)
+      let nraenv_of_from_clause :=
+          fold_left nraenv_of_from from_clause (NRAEnvUnop AColl NRAEnvID)
       in
-      let algenv_of_where_clause :=
+      let nraenv_of_where_clause :=
           match where_clause with
-          | OTrue => algenv_of_from_clause
+          | OTrue => nraenv_of_from_clause
           | OWhere where_expr =>
-            ANSelect (algenv_of_oql where_expr) algenv_of_from_clause
+            NRAEnvSelect (nraenv_of_oql where_expr) nraenv_of_from_clause
           end
       in
-      let algenv_of_order_clause :=
+      let nraenv_of_order_clause :=
           match order_clause with
-          | ONoOrder => algenv_of_where_clause
-          | OOrderBy e sc => algenv_of_where_clause
+          | ONoOrder => nraenv_of_where_clause
+          | OOrderBy e sc => nraenv_of_where_clause
           end
       in
       match select_clause with
       | OSelect select_expr =>
-        ANMap (algenv_of_oql select_expr) algenv_of_order_clause
+        NRAEnvMap (nraenv_of_oql select_expr) nraenv_of_order_clause
       | OSelectDistinct select_expr =>
-        ANUnop ADistinct (ANMap (algenv_of_oql select_expr) algenv_of_order_clause)
+        NRAEnvUnop ADistinct (NRAEnvMap (nraenv_of_oql select_expr) nraenv_of_order_clause)
       end
     end.
 
@@ -301,11 +300,11 @@ Section OQLtoNRAEnv.
    * Select clause correctness *
    *****************************)
   
-  Lemma algenv_of_select_expr_correct
+  Lemma nraenv_of_select_expr_correct
         (o:oql_expr) (xenv:data) (env0 : option (list oql_env)) :
     (forall (xenv : data) (env : oql_env),
         oql_interp h constant_env o env =
-        (h ⊢ₑ algenv_of_oql o @ₑ (drec env) ⊣ constant_env; xenv )%algenv) ->
+        (h ⊢ nraenv_of_oql o @ₓ (drec env) ⊣ constant_env; xenv )%nraenv) ->
     olift (fun x0 : list oql_env => lift dcoll (rmap (oql_interp h constant_env o) x0)) env0 =
     olift
       (fun d : data =>
@@ -313,17 +312,17 @@ Section OQLtoNRAEnv.
            (fun c1 : list data =>
               lift dcoll
                    (rmap
-                      (fun_of_algenv h constant_env (algenv_of_oql o) xenv)
+                      (nraenv_eval h constant_env (nraenv_of_oql o) xenv)
                       c1)) d) (lift (fun x => dcoll (map drec x)) env0).
   Proof.
     intros.
     destruct env0; [|reflexivity]; simpl.
     induction l; simpl; try reflexivity.
     rewrite (H xenv).
-    destruct (h ⊢ₑ algenv_of_oql o @ₑ (drec a) ⊣ constant_env; xenv)%algenv; simpl;
+    destruct (h ⊢ nraenv_of_oql o @ₓ (drec a) ⊣ constant_env; xenv)%nraenv; simpl;
     [|reflexivity].
     destruct (rmap (oql_interp h constant_env o) l);
-      destruct (rmap (fun_of_algenv h constant_env (algenv_of_oql o) xenv)
+      destruct (rmap (nraenv_eval h constant_env (nraenv_of_oql o) xenv)
                      (map drec l)); simpl in *; congruence.
   Qed.
 
@@ -336,13 +335,12 @@ Section OQLtoNRAEnv.
      variable and does cartesian product (i.e., MapConcat) *)
 
   Lemma one_from_fold_step_is_map_concat s o op xenv envs envs0:
-    (h ⊢ₑ op @ₑ envs ⊣ constant_env; xenv)%algenv =
+    (h ⊢ op @ₓ envs ⊣ constant_env; xenv)%nraenv =
     lift (fun x : list (list (string * data)) => dcoll (map drec x)) envs0 ->
     (forall (xenv0 : data) (env : oql_env),
        oql_interp h constant_env o env =
-       (h ⊢ₑ algenv_of_oql o @ₑ drec env ⊣ constant_env; xenv0)%algenv) ->
-    ((h ⊢ₑ (⋈ᵈ⟨χ⟨‵[| (s, ID)|] ⟩( algenv_of_oql o) ⟩( op))%algenv
-        @ₑ envs ⊣ constant_env; xenv)%algenv =
+       (h ⊢ nraenv_of_oql o @ₓ drec env ⊣ constant_env; xenv0)%nraenv) ->
+    ((h ⊢ (NRAEnvMapConcat (NRAEnvMap (NRAEnvUnop (ARec s) NRAEnvID) (nraenv_of_oql o)) op) @ₓ envs ⊣ constant_env; xenv)%nraenv =
      lift (fun x : list (list (string * data)) => dcoll (map drec x))
           (match envs0 with
            | Some envl' =>
@@ -351,6 +349,7 @@ Section OQLtoNRAEnv.
            end)).
   Proof.
     intros; simpl.
+    unfold nraenv_eval in *; simpl.
     rewrite H; simpl; clear H.
     destruct envs0; [|reflexivity]; simpl.
     induction l; try reflexivity; simpl.
@@ -359,7 +358,9 @@ Section OQLtoNRAEnv.
     unfold oomap_concat in *; simpl.
     unfold oenv_map_concat_single in *; simpl.
     rewrite (H0 xenv).
-    destruct (h ⊢ₑ algenv_of_oql o @ₑ drec a ⊣ constant_env; xenv)%algenv;
+    destruct (RAlgEnv.fun_of_algenv h constant_env
+          (algenv_of_nraenv (nraenv_of_oql o)) xenv 
+          (drec a))%nraenv;
       try reflexivity; simpl.
     destruct d; try reflexivity; simpl.
     autorewrite with alg; simpl.
@@ -385,7 +386,8 @@ Section OQLtoNRAEnv.
                         (rmap
                            (fun x : data => Some (drec ((s, x) :: nil)))
                            c1)) d)
-                  (h ⊢ₑ algenv_of_oql o @ₑ a0 ⊣ constant_env; xenv)%algenv
+                  (RAlgEnv.fun_of_algenv h constant_env
+                  (algenv_of_nraenv (nraenv_of_oql o)) xenv a0)%nraenv
               with
               | Some (dcoll y) => rmap (fun x : data => orecconcat a0 x) y
               | Some _ => None
@@ -402,16 +404,20 @@ Section OQLtoNRAEnv.
      MapConcat) as well *)
 
   Lemma one_from_cast_fold_step_is_map_concat_cast s bn o op xenv envs envs0:
-    (h ⊢ₑ op @ₑ envs ⊣ constant_env; xenv)%algenv =
+    (h ⊢ op @ₓ envs ⊣ constant_env; xenv)%nraenv =
     lift (fun x : list (list (string * data)) => dcoll (map drec x)) envs0 ->
     (forall (xenv0 : data) (env : oql_env),
        oql_interp h constant_env o env =
-       (h ⊢ₑ algenv_of_oql o @ₑ drec env ⊣ constant_env; xenv0)%algenv) ->
-    ((h ⊢ₑ (⋈ᵈ⟨ χ⟨ ‵[| (s, ID) |]
-                 ⟩( ♯flatten( χ⟨ ANEither (‵{| ID|}) ‵{||}
-                               ⟩( χ⟨ ANUnop (ACast (bn :: nil)) (ID)
-                                   ⟩( algenv_of_oql o)))) ⟩( op)) @ₑ envs
-        ⊣ constant_env; xenv)%algenv
+       (h ⊢ nraenv_of_oql o @ₓ drec env ⊣ constant_env; xenv0)%nraenv) ->
+    ((h ⊢ (NRAEnvMapConcat
+             (NRAEnvMap
+                (NRAEnvUnop (ARec s) NRAEnvID)
+                (NRAEnvUnop AFlatten(
+                              NRAEnvMap (NRAEnvEither (NRAEnvUnop AColl NRAEnvID)
+                                                      (NRAEnvConst (dcoll nil)))
+                                        (NRAEnvMap (NRAEnvUnop (ACast (bn :: nil)) NRAEnvID)
+                                                   (nraenv_of_oql o))))) op) @ₓ envs
+        ⊣ constant_env; xenv)%nraenv
      =
      lift (fun x : list (list (string * data)) => dcoll (map drec x))
           match envs0 with
@@ -421,6 +427,7 @@ Section OQLtoNRAEnv.
           end).
   Proof.
     intros; simpl.
+    unfold nraenv_eval in *; simpl.
     rewrite H; simpl; clear H.
     destruct envs0; [|reflexivity]; simpl.
     induction l; try reflexivity; simpl.
@@ -429,7 +436,9 @@ Section OQLtoNRAEnv.
     unfold oomap_concat in *; simpl.
     unfold oenv_map_concat_single_with_cast in *; simpl.
     rewrite (H0 xenv).
-    destruct (h ⊢ₑ algenv_of_oql o @ₑ drec a ⊣ constant_env; xenv)%algenv;
+    destruct (RAlgEnv.fun_of_algenv h constant_env
+          (algenv_of_nraenv (nraenv_of_oql o)) xenv 
+          (drec a))%nraenv;
       try reflexivity; simpl.
     destruct d; try reflexivity; simpl.
     unfold filter_cast in *; simpl in *.
@@ -792,7 +801,8 @@ Section OQLtoNRAEnv.
                                          else Some dnone
                                      | dforeign _ => None
                                      end) c1)) d)
-                           (h ⊢ₑ algenv_of_oql o @ₑ a ⊣ constant_env; xenv)%algenv)))
+                           (RAlgEnv.fun_of_algenv h constant_env
+                              (algenv_of_nraenv (nraenv_of_oql o)) xenv a)%nraenv)))
               with
               | Some dunit => None
               | Some (dnat _) => None
@@ -868,7 +878,8 @@ Section OQLtoNRAEnv.
                                                  else Some dnone
                                                | dforeign _ => None
                                                end) c1)) d)
-                            (h ⊢ₑ algenv_of_oql o @ₑ a ⊣ constant_env; xenv)%algenv)))
+                            (RAlgEnv.fun_of_algenv h constant_env
+                              (algenv_of_nraenv (nraenv_of_oql o)) xenv a))))
                with
                | Some dunit => None
                | Some (dnat _) => None
@@ -886,21 +897,25 @@ Section OQLtoNRAEnv.
 
   (* Second, show that 'x in expr' translation is correct *)
   
-  Lemma algenv_of_from_in_correct env o s xenv :
+  Lemma nraenv_of_from_in_correct env o s xenv :
     (forall (xenv0 : data) (env0 : oql_env),
         oql_interp h constant_env o env0 =
-        (h ⊢ₑ algenv_of_oql o @ₑ drec env0 ⊣ constant_env; xenv0)%algenv) ->
+        (h ⊢ nraenv_of_oql o @ₓ drec env0 ⊣ constant_env; xenv0)%nraenv) ->
     (lift (fun x : list (list (string * data)) => dcoll (map drec x))
           (env_map_concat s (oql_interp h constant_env o) (env :: nil))) =
-    (fun_of_algenv h constant_env (ANMapConcat (ANMap (ANUnop (ARec s) ANID) (algenv_of_oql o)) (ANUnop AColl ANID)) xenv (drec env)).
+    (nraenv_eval h constant_env (NRAEnvMapConcat (NRAEnvMap (NRAEnvUnop (ARec s) NRAEnvID) (nraenv_of_oql o)) (NRAEnvUnop AColl NRAEnvID)) xenv (drec env)).
   Proof.
     intros; simpl.
+    unfold nraenv_eval; simpl.
     unfold rmap_concat; simpl.
     unfold env_map_concat; simpl.
     unfold oomap_concat; simpl.
     unfold oenv_map_concat_single; simpl.
     rewrite (H xenv); clear H.
-    destruct (h ⊢ₑ algenv_of_oql o @ₑ drec env ⊣ constant_env; xenv)%algenv;
+    unfold nraenv_eval; simpl.
+    destruct (RAlgEnv.fun_of_algenv h constant_env
+          (algenv_of_nraenv (nraenv_of_oql o)) xenv 
+          (drec env))%nraenv;
       try reflexivity; simpl.
     destruct d; simpl; try reflexivity.
     autorewrite with alg; simpl.
@@ -910,14 +925,14 @@ Section OQLtoNRAEnv.
 
   (* Finally, the main fold_left for a whole from clause is correct *)
   
-  Lemma algenv_of_from_clause_correct op envs envs0 el xenv :
+  Lemma nraenv_of_from_clause_correct op envs envs0 el xenv :
     Forall
       (fun ab : oql_in_expr =>
          forall (xenv : data) (env : oql_env),
            oql_interp h constant_env (oin_expr ab) env =
-           (h ⊢ₑ algenv_of_oql (oin_expr ab) @ₑ drec env ⊣ constant_env;
-             xenv)%algenv) el ->
-    (h ⊢ₑ op @ₑ envs ⊣ constant_env; xenv)%algenv =
+           (h ⊢ nraenv_of_oql (oin_expr ab) @ₓ drec env ⊣ constant_env;
+             xenv)%nraenv) el ->
+    (h ⊢ op @ₓ envs ⊣ constant_env; xenv)%nraenv =
     (lift (fun x : list (list (string * data)) => dcoll (map drec x)) envs0) ->
     (lift (fun x : list (list (string * data)) => dcoll (map drec x))
           (fold_left
@@ -939,19 +954,27 @@ Section OQLtoNRAEnv.
           end
              ) el envs0)) =
     (h
-       ⊢ₑ fold_left
-       (fun (opacc : algenv) (from_in_expr : oql_in_expr) =>
+       ⊢ fold_left
+       (fun (opacc : nraenv) (from_in_expr : oql_in_expr) =>
           match from_in_expr with
           | OIn in_v from_expr =>
-            ⋈ᵈ⟨χ⟨‵[| (in_v, ID)|] ⟩( algenv_of_oql from_expr) ⟩(opacc)
+            NRAEnvMapConcat
+              (NRAEnvMap (NRAEnvUnop (ARec in_v) NRAEnvID) (nraenv_of_oql from_expr))
+              opacc
           | OInCast in_v brand_name from_expr =>
-            ⋈ᵈ⟨χ⟨‵[| (in_v, ID)|] ⟩(
-                  ♯flatten(χ⟨ ANEither (ANUnop AColl ANID)
-                              (ANConst (dcoll nil)) ⟩(
-                     χ⟨ ANUnop (ACast (brand_name::nil)) ANID ⟩(algenv_of_oql from_expr)))) ⟩(opacc)
+            NRAEnvMapConcat
+              (NRAEnvMap
+                 (NRAEnvUnop (ARec in_v) NRAEnvID)
+                 (NRAEnvUnop AFlatten
+                             (NRAEnvMap (NRAEnvEither (NRAEnvUnop AColl NRAEnvID)
+                                                      (NRAEnvConst (dcoll nil)))
+                                        (NRAEnvMap (NRAEnvUnop (ACast (brand_name::nil))
+                                                               NRAEnvID)
+                                                   (nraenv_of_oql from_expr)))))
+              opacc
           end
        )
-       el op @ₑ envs ⊣ constant_env; xenv)%algenv.
+       el op @ₓ envs ⊣ constant_env; xenv)%nraenv.
   Proof.
     intros.
     revert op xenv envs0 envs H0.
@@ -960,9 +983,13 @@ Section OQLtoNRAEnv.
     (* OIn case *)
     - inversion H; subst; simpl in *.
       specialize (IHel H4); clear H H4.
-      specialize (IHel (⋈ᵈ⟨χ⟨‵[| (s, ID)|] ⟩( algenv_of_oql o) ⟩( op))%algenv).
-      assert ((h ⊢ₑ (⋈ᵈ⟨χ⟨‵[| (s, ID)|] ⟩( algenv_of_oql o) ⟩( op))%algenv
-                 @ₑ envs ⊣ constant_env; xenv)%algenv =
+      specialize (IHel (NRAEnvMapConcat
+                          (NRAEnvMap (NRAEnvUnop (ARec s) NRAEnvID)
+                                     (nraenv_of_oql o)) op)%nraenv).
+      assert ((h ⊢ (NRAEnvMapConcat
+                      (NRAEnvMap (NRAEnvUnop (ARec s) NRAEnvID)
+                                 (nraenv_of_oql o)) op)%nraenv
+                 @ₓ envs ⊣ constant_env; xenv)%nraenv =
               lift (fun x : list (list (string * data)) => dcoll (map drec x))
                    (match envs0 with
                     | Some envl' =>
@@ -978,15 +1005,26 @@ Section OQLtoNRAEnv.
     (* OInCast case *)
     - inversion H; subst; simpl in *.
       specialize (IHel H4); clear H H4.
-      specialize (IHel (⋈ᵈ⟨ χ⟨ ‵[| (s, ID) |]
-                          ⟩( ♯flatten( χ⟨ ANEither (‵{| ID|}) ‵{||}
-                                        ⟩( χ⟨ ANUnop (ACast (s0 :: nil)) (ID)
-                                            ⟩( algenv_of_oql o)))) ⟩( op))%algenv).
-      assert ((h ⊢ₑ (⋈ᵈ⟨ χ⟨ ‵[| (s, ID) |]
-                          ⟩( ♯flatten( χ⟨ ANEither (‵{| ID|}) ‵{||}
-                                        ⟩( χ⟨ ANUnop (ACast (s0 :: nil)) (ID)
-                                            ⟩( algenv_of_oql o)))) ⟩( op)) @ₑ envs
-                 ⊣ constant_env; xenv)%algenv
+      specialize
+        (IHel (NRAEnvMapConcat
+                 (NRAEnvMap
+                    (NRAEnvUnop (ARec s) NRAEnvID)
+                    (NRAEnvUnop AFlatten
+                                (NRAEnvMap
+                                   (NRAEnvEither (NRAEnvUnop AColl NRAEnvID)
+                                                 (NRAEnvConst (dcoll nil)))
+                                   (NRAEnvMap (NRAEnvUnop (ACast (s0 :: nil)) NRAEnvID)
+                                              (nraenv_of_oql o))))) (op))%nraenv).
+      assert ((h ⊢ (NRAEnvMapConcat
+                 (NRAEnvMap
+                    (NRAEnvUnop (ARec s) NRAEnvID)
+                    (NRAEnvUnop AFlatten
+                                (NRAEnvMap
+                                   (NRAEnvEither (NRAEnvUnop AColl NRAEnvID)
+                                                 (NRAEnvConst (dcoll nil)))
+                                   (NRAEnvMap (NRAEnvUnop (ACast (s0 :: nil)) NRAEnvID)
+                                              (nraenv_of_oql o))))) (op)) @ₓ envs
+                 ⊣ constant_env; xenv)%nraenv
               =
               lift (fun x : list (list (string * data)) => dcoll (map drec x))
                    match envs0 with
@@ -1006,11 +1044,11 @@ Section OQLtoNRAEnv.
    * Where clause correctness *
    ****************************)
   
-  Lemma algenv_of_where_clause_correct
+  Lemma nraenv_of_where_clause_correct
         (o:oql_expr) (xenv:data) (ol : option (list oql_env)):
     (forall (xenv : data) (env : oql_env),
         oql_interp h constant_env o env =
-        (h ⊢ₑ algenv_of_oql o @ₑ drec env ⊣ constant_env; xenv)%algenv) ->
+        (h ⊢ nraenv_of_oql o @ₓ drec env ⊣ constant_env; xenv)%nraenv) ->
     lift (fun x : list (list (string * data)) => dcoll (map drec x))
          (olift
             (lift_filter
@@ -1028,7 +1066,7 @@ Section OQLtoNRAEnv.
                    (lift_filter
                       (fun x' : data =>
                          match
-                           (h ⊢ₑ algenv_of_oql o @ₑ x' ⊣ constant_env; xenv)%algenv
+                           (h ⊢ nraenv_of_oql o @ₓ x' ⊣ constant_env; xenv)%nraenv
                          with
                          | Some (dbool b) => Some b
                          | Some _ => None
@@ -1040,12 +1078,12 @@ Section OQLtoNRAEnv.
     destruct ol; [|reflexivity]; simpl.
     induction l; [reflexivity|idtac]; simpl.
     rewrite (H xenv a); simpl in *.
-    destruct (h ⊢ₑ algenv_of_oql o @ₑ drec a ⊣ constant_env; xenv)%algenv; try reflexivity; simpl.
+    destruct (h ⊢ nraenv_of_oql o @ₓ drec a ⊣ constant_env; xenv)%nraenv; try reflexivity; simpl.
     destruct d; try reflexivity; simpl.
     destruct (lift_filter
              (fun x' : data =>
               match
-                (h ⊢ₑ algenv_of_oql o @ₑ x' ⊣ constant_env; xenv)%algenv
+                (h ⊢ nraenv_of_oql o @ₓ x' ⊣ constant_env; xenv)%nraenv
               with
               | Some (dbool b0) => Some b0
               | Some _ => None
@@ -1063,10 +1101,10 @@ Section OQLtoNRAEnv.
 
   (* Main theorem: OQL to NRAEnv translation is correct *)
   
-  Theorem algenv_of_oql_correct (e:oql_expr) :
+  Theorem nraenv_of_oql_correct (e:oql_expr) :
     forall xenv:data, forall env:oql_env,
         oql_interp h constant_env e env =
-        fun_of_algenv h constant_env (algenv_of_oql e) xenv (drec env).
+        nraenv_eval h constant_env (nraenv_of_oql e) xenv (drec env).
   Proof.
     intros. revert xenv env.
     induction e; simpl; intros.
@@ -1085,49 +1123,89 @@ Section OQLtoNRAEnv.
     (* OSFW *)
     - destruct e1.
       + simpl in *.
-        rewrite <- (algenv_of_from_clause_correct _ _ (Some (env :: nil))) ; [idtac|assumption|reflexivity].
-        rewrite <- algenv_of_select_expr_correct; [|assumption].
+        generalize nraenv_of_from_clause_correct; intros Hfrom.
+        unfold nraenv_eval in *; simpl.
+        rewrite <- (Hfrom _ _ (Some (env :: nil))) ; [idtac|assumption|reflexivity].
+        generalize nraenv_of_select_expr_correct; intros Hselect.
+        unfold nraenv_eval in *; simpl.
+        rewrite <- Hselect; [|assumption].
         reflexivity.
       + simpl in *.
-        rewrite <- (algenv_of_from_clause_correct _ _ (Some (env :: nil))) ; [idtac|assumption|reflexivity].
-        rewrite <- algenv_of_select_expr_correct; [|assumption].
+        generalize nraenv_of_from_clause_correct; intros Hfrom.
+        unfold nraenv_eval in *; simpl.
+        rewrite <- (Hfrom _ _ (Some (env :: nil))) ; [idtac|assumption|reflexivity].
+        generalize nraenv_of_select_expr_correct; intros Hselect.
+        unfold nraenv_eval in *; simpl.
+        rewrite <- Hselect; [|assumption].
         rewrite push_lift_coll_in_rmap; simpl.
         rewrite olift_rondcoll_over_dcoll.
         reflexivity.
     - destruct e1.
       + simpl in *.
-        rewrite <- (algenv_of_from_clause_correct _ _ (Some (env :: nil))) ; [idtac|assumption|reflexivity]. 
-        rewrite <- algenv_of_where_clause_correct; [|assumption].
-        rewrite <- algenv_of_select_expr_correct; [|assumption].
+        generalize nraenv_of_from_clause_correct; intros Hfrom.
+        unfold nraenv_eval in *; simpl.
+        rewrite <- (Hfrom _ _ (Some (env :: nil))) ; [idtac|assumption|reflexivity]. 
+        generalize nraenv_of_where_clause_correct; intros Hwhere.
+        unfold nraenv_eval in *; simpl.
+        rewrite <- Hwhere; [|assumption].
+        generalize nraenv_of_select_expr_correct; intros Hselect.
+        unfold nraenv_eval in *; simpl.
+        rewrite <- Hselect; [|assumption].
         reflexivity.
       + simpl in *.
-        rewrite <- (algenv_of_from_clause_correct _ _ (Some (env :: nil))) ; [idtac|assumption|reflexivity].
-        rewrite <- algenv_of_where_clause_correct; [|assumption].
-        rewrite <- algenv_of_select_expr_correct; [|assumption].
+        generalize nraenv_of_from_clause_correct; intros Hfrom.
+        unfold nraenv_eval in *; simpl.
+        rewrite <- (Hfrom _ _ (Some (env :: nil))) ; [idtac|assumption|reflexivity]. 
+        generalize nraenv_of_where_clause_correct; intros Hwhere.
+        unfold nraenv_eval in *; simpl.
+        rewrite <- Hwhere; [|assumption].
+        generalize nraenv_of_select_expr_correct; intros Hselect.
+        unfold nraenv_eval in *; simpl.
+        rewrite <- Hselect; [|assumption].
         rewrite push_lift_coll_in_rmap; simpl.
         rewrite olift_rondcoll_over_dcoll.
         reflexivity.
     - destruct e1.
       + simpl in *.
-        rewrite <- (algenv_of_from_clause_correct _ _ (Some (env :: nil))) ; [idtac|assumption|reflexivity].
-        rewrite <- algenv_of_select_expr_correct; [|assumption].
+        generalize nraenv_of_from_clause_correct; intros Hfrom.
+        unfold nraenv_eval in *; simpl.
+        rewrite <- (Hfrom _ _ (Some (env :: nil))) ; [idtac|assumption|reflexivity]. 
+        generalize nraenv_of_select_expr_correct; intros Hselect.
+        unfold nraenv_eval in *; simpl.
+        rewrite <- Hselect; [|assumption].
         reflexivity.
       + simpl in *.
-        rewrite <- (algenv_of_from_clause_correct _ _ (Some (env :: nil))) ; [idtac|assumption|reflexivity].
-        rewrite <- algenv_of_select_expr_correct; [|assumption].
+        generalize nraenv_of_from_clause_correct; intros Hfrom.
+        unfold nraenv_eval in *; simpl.
+        rewrite <- (Hfrom _ _ (Some (env :: nil))) ; [idtac|assumption|reflexivity]. 
+        generalize nraenv_of_select_expr_correct; intros Hselect.
+        unfold nraenv_eval in *; simpl.
+        rewrite <- Hselect; [|assumption].
         rewrite push_lift_coll_in_rmap; simpl.
         rewrite olift_rondcoll_over_dcoll.
         reflexivity.
     - destruct e1.
       + simpl in *.
-        rewrite <- (algenv_of_from_clause_correct _ _ (Some (env :: nil))) ; [idtac|assumption|reflexivity]. 
-        rewrite <- algenv_of_where_clause_correct; [|assumption].
-        rewrite <- algenv_of_select_expr_correct; [|assumption].
+        generalize nraenv_of_from_clause_correct; intros Hfrom.
+        unfold nraenv_eval in *; simpl.
+        rewrite <- (Hfrom _ _ (Some (env :: nil))) ; [idtac|assumption|reflexivity]. 
+        generalize nraenv_of_where_clause_correct; intros Hwhere.
+        unfold nraenv_eval in *; simpl.
+        rewrite <- Hwhere; [|assumption].
+        generalize nraenv_of_select_expr_correct; intros Hselect.
+        unfold nraenv_eval in *; simpl.
+        rewrite <- Hselect; [|assumption].
         reflexivity.
       + simpl in *.
-        rewrite <- (algenv_of_from_clause_correct _ _ (Some (env :: nil))) ; [idtac|assumption|reflexivity].
-        rewrite <- algenv_of_where_clause_correct; [|assumption].
-        rewrite <- algenv_of_select_expr_correct; [|assumption].
+        generalize nraenv_of_from_clause_correct; intros Hfrom.
+        unfold nraenv_eval in *; simpl.
+        rewrite <- (Hfrom _ _ (Some (env :: nil))) ; [idtac|assumption|reflexivity]. 
+        generalize nraenv_of_where_clause_correct; intros Hwhere.
+        unfold nraenv_eval in *; simpl.
+        rewrite <- Hwhere; [|assumption].
+        generalize nraenv_of_select_expr_correct; intros Hselect.
+        unfold nraenv_eval in *; simpl.
+        rewrite <- Hselect; [|assumption].
         rewrite push_lift_coll_in_rmap; simpl.
         rewrite olift_rondcoll_over_dcoll.
         reflexivity.
@@ -1135,9 +1213,9 @@ Section OQLtoNRAEnv.
 
   (* Top-level translation call *)
 
-  Definition translate_oql_to_algenv (e:oql_expr) : algenv :=
+  Definition translate_oql_to_nraenv (e:oql_expr) : nraenv :=
     (* Produces the initial plan *)
-    ANApp (algenv_of_oql e) (ANConst (drec nil)).
+    NRAEnvApp (nraenv_of_oql e) (NRAEnvConst (drec nil)).
 
   (********************************************
    * Additional properties of the translation *
@@ -1145,23 +1223,29 @@ Section OQLtoNRAEnv.
   
   (* OQL to NRAEnv translation is local env-free *)
 
-  Require Import RAlgEnvIgnore.
-
   (* For fold_left, make sure to do the induction on el for *any* accumulator *)
-  Lemma fold_left_ignore_env (el:list oql_in_expr) (a:algenv) :
-    ignores_env a ->
-    Forall (fun ab : oql_in_expr => ignores_env (algenv_of_oql (oin_expr ab))) el ->
-    ignores_env
+  Lemma fold_left_ignore_env (el:list oql_in_expr) (a:nraenv) :
+    nraenv_ignores_env a ->
+    Forall (fun ab : oql_in_expr => nraenv_ignores_env (nraenv_of_oql (oin_expr ab))) el ->
+    nraenv_ignores_env
       (fold_left
-         (fun (opacc : algenv) (from_in_expr : oql_in_expr) =>
+         (fun (opacc : nraenv) (from_in_expr : oql_in_expr) =>
             match from_in_expr with
             | OIn in_v from_expr =>
-              (⋈ᵈ⟨χ⟨‵[| (in_v, ID)|] ⟩( algenv_of_oql from_expr) ⟩( opacc))%algenv
+              (NRAEnvMapConcat
+                 (NRAEnvMap
+                    (NRAEnvUnop (ARec in_v) NRAEnvID)
+                    (nraenv_of_oql from_expr)) opacc)%nraenv
             | OInCast in_v brand_name from_expr =>
-              ⋈ᵈ⟨χ⟨‵[| (in_v, ID)|] ⟩(
-                  ♯flatten(χ⟨ ANEither (ANUnop AColl ANID)
-                              (ANConst (dcoll nil)) ⟩(
-                     χ⟨ ANUnop (ACast (brand_name::nil)) ANID ⟩(algenv_of_oql from_expr)))) ⟩(opacc)%algenv
+             (NRAEnvMapConcat
+                (NRAEnvMap (NRAEnvUnop (ARec in_v) NRAEnvID)
+                           (NRAEnvUnop AFlatten
+                                       (NRAEnvMap
+                                          (NRAEnvEither (NRAEnvUnop AColl NRAEnvID)
+                                                        (NRAEnvConst (dcoll nil)))
+                                          (NRAEnvMap
+                                             (NRAEnvUnop (ACast (brand_name::nil)) NRAEnvID)
+                                             (nraenv_of_oql from_expr))))) opacc)%nraenv
             end)
          el a).
   Proof.
@@ -1172,19 +1256,24 @@ Section OQLtoNRAEnv.
     specialize (IHel H4); clear H4.
     destruct a; simpl in *.
     - apply IHel.
+      unfold nraenv_ignores_env.
       simpl; auto.
     - apply IHel.
+      unfold nraenv_ignores_env.
       simpl; auto.
   Qed.
     
   Lemma oql_to_nraenv_ignores_env (e:oql_expr) :
-    ignores_env (algenv_of_oql e).
+    nraenv_ignores_env (nraenv_of_oql e).
   Proof.
-    induction e; simpl; auto;
+    induction e; simpl;
+    unfold nraenv_ignores_env; simpl;
+    auto;
     destruct e1;
     simpl in *;
     repeat (split; auto);
-    apply fold_left_ignore_env; simpl; auto.
+    apply fold_left_ignore_env; unfold nraenv_ignores_env;
+    simpl; auto.
   Qed.
 
 End OQLtoNRAEnv.
