coq/Compiler/QLib/QDriver.v
@@ -84,20 +84,11 @@ Module QDriver(runtime:CompilerRuntime).
     Definition nraenv_core_optim_to_nnrc_optim_to_nnrcmr_comptop_optim : nraenv_core -> nrcmr
       := nraenv_core_optim_to_nnrc_optim_to_nnrcmr_comptop_optim.
 
-    (* Used in FrontUtil: *)
-    Definition rule_to_nraenv_core := rule_to_nraenv_core.
-    Definition rule_to_camp := rule_to_camp.
-    Definition camp_to_nraenv_core := camp_to_nraenv_core.
-    Definition oql_to_nraenv_core := oql_to_nraenv_core.
-
     (* Used in CloudantUtil *)
     Definition cldmr_to_cloudant : string -> list (string*string) -> cldmr -> cloudant := cldmr_to_cloudant.
     Definition nnrcmr_to_cldmr : list (string*string) -> nnrcmr -> cldmr := nnrcmr_to_cldmr.
     Definition nnrcmr_prepared_to_cldmr : list (string*string) -> nnrcmr -> cldmr := nnrcmr_prepared_to_cldmr.
 
-    (* Used in EvalUtil *)
-    Definition nraenv_core_optim := nraenv_core_optim.
-    
     (* Used in queryTests: *)
     Definition rule_to_nraenv_core_to_nnrc_optim : rule -> nnrc := rule_to_nraenv_core_to_nnrc_optim.
     Definition rule_to_nraenv_core_to_nnrc_optim_to_dnnrc :
